theories/Spilling/Spilling.v
@@ -32,7 +32,7 @@ ann (set var * set var * option (list (set var * set var)))
 
 | SpillApp ZL Z Λ R M Sp L K f Y R_f M_f
 : cardinal (R\K ∪ L) <= k
-  -> list_union (Op.freeVars ⊝ Y) ⊆ R\K ∪ L
+  (*-> list_union (Op.freeVars ⊝ Y) ⊆ R\K ∪ L*)
   -> get ZL (counted f) Z
   -> get Λ (counted f) (R_f,M_f)
   -> R_f \ of_list Z ⊆ R\K ∪ L
@@ -42,13 +42,12 @@ ann (set var * set var * option (list (set var * set var)))
 | SpillFun (ZL:list params) Λ R M Sp L K t sl_F sl_t (F: list(params*stmt)) rms
 : cardinal (R\K ∪ L) <= k
   -> (forall n rm, get rms n rm -> cardinal (fst rm) <= k)
-  (*-> R_f ⊆ R\K ∪ Sp ∪ M ∪ of_list Z
-  -> M_f ⊆ R\K ∪ Sp ∪ M ∪ of_list Z*)
   -> (forall n Zs rm sl_s, get rms n rm
      -> get F n Zs
      -> get sl_F n sl_s
-     -> spill_sound k ((List.map fst F) ++ ZL) (rms ++ Λ) rm (snd Zs) sl_s)
-  -> spill_sound k ((List.map fst F) ++ ZL) (rms ++ Λ) (R\K ∪ L, Sp ∪ M) t sl_t
+     -> spill_sound k ((fst ⊝ F) ++ ZL) (rms ++ Λ) rm (snd Zs) sl_s
+     )
+  -> spill_sound k ((fst ⊝ F) ++ ZL) (rms ++ Λ) (R\K ∪ L, Sp ∪ M) t sl_t
     -> spill_sound k ZL Λ (R,M) (stmtFun F t)
                    (annF (Sp,L,Some rms) sl_F sl_t)
 .
